verif/btrees/verif_newnode.v
@@ -3,9 +3,6 @@
 Require Import VST.floyd.proofauto.
 Require Import VST.floyd.library.
 Require Import relation_mem.
-Instance CompSpecs : compspecs. make_compspecs prog. Defined.
-Definition Vprog : varspecs. mk_varspecs prog. Defined.
-
 Require Import VST.msl.wand_frame.
 Require Import VST.msl.iter_sepcon.
 Require Import VST.floyd.reassoc_seq.
@@ -38,5 +35,4 @@ Proof.
       Exists vret. entailer!.
       Exists (list_repeat 15 (Vundef, (inl Vundef):(val+val))).
       simpl. cancel.
-      apply derives_refl.
 Qed.
